@prefix : <http://example.org/def/production-trace-patterns/> .
@prefix owl: <http://www.w3.org/2002/07/owl#> .
@prefix rdf: <http://www.w3.org/1999/02/22-rdf-syntax-ns#> .
@prefix xml: <http://www.w3.org/XML/1998/namespace> .
@prefix xsd: <http://www.w3.org/2001/XMLSchema#> .
@prefix rdfs: <http://www.w3.org/2000/01/rdf-schema#> .
@base <http://example.org/def/production-trace-patterns/> .

<http://example.org/def/production-trace-patterns/> rdf:type owl:Ontology .

#################################################################
#    Object Properties
#################################################################

###  http://example.org/def/production-trace-patterns/entity
:entity rdf:type owl:ObjectProperty ;
        rdfs:subPropertyOf owl:topObjectProperty ;
        rdfs:domain :Event ;
        rdfs:range :Event .


###  http://example.org/def/production-trace-patterns/isPartOf
:isPartOf rdf:type owl:ObjectProperty ;
          rdfs:domain :Entity ;
          rdfs:range :Entity .


###  http://example.org/def/production-trace-patterns/state
:state rdf:type owl:ObjectProperty ;
       rdfs:domain :SwitchState ;
       rdfs:range :State .


#################################################################
#    Data properties
#################################################################

###  http://example.org/def/production-trace-patterns/atTime
:atTime rdf:type owl:DatatypeProperty ;
        rdfs:domain :Event ;
        rdfs:range xsd:dateTime .


#################################################################
#    Classes
#################################################################

###  http://example.org/def/production-trace-patterns/AGV
:AGV rdf:type owl:Class ;
     rdfs:subClassOf :Resource ;
     rdfs:comment "Automated Guided Vehicle that can be used to transport objects (e.g. products and materials) between locations in a manufacturing environment."@en .


###  http://example.org/def/production-trace-patterns/Alarm
:Alarm rdf:type owl:Class ;
       rdfs:subClassOf :Event ;
       rdfs:comment "Describes the occasion when a Resource has some issue and raises a warning."@en .


###  http://example.org/def/production-trace-patterns/Buffer
:Buffer rdf:type owl:Class ;
        rdfs:subClassOf :Resource ;
        rdfs:comment "Resource where objects are temporarily stored, for example a product can be stored in a buffer in front of a machine while the machine is processing another product."@en .


###  http://example.org/def/production-trace-patterns/Component
:Component rdf:type owl:Class ;
           rdfs:subClassOf :Product ;
           rdfs:comment "A part of the Product, for example a sub-assembly."@en .


###  http://example.org/def/production-trace-patterns/Consume
:Consume rdf:type owl:Class ;
         rdfs:subClassOf :Event ;
         rdfs:comment "Describes the occasion when objects are used to produce something else, for example during the assembly of a Component to a Product."@en .


###  http://example.org/def/production-trace-patterns/Entity
:Entity rdf:type owl:Class ;
        rdfs:comment "Thing or object, not necessary physical."@en .


###  http://example.org/def/production-trace-patterns/Event
:Event rdf:type owl:Class ;
       rdfs:comment "Occasion or something that happens, which is the effect of a process that is executed."@en .


###  http://example.org/def/production-trace-patterns/Failed
:Failed rdf:type owl:Class ;
        rdfs:subClassOf :State .


###  http://example.org/def/production-trace-patterns/Idle
:Idle rdf:type owl:Class ;
      rdfs:subClassOf :State .


###  http://example.org/def/production-trace-patterns/Job
:Job rdf:type owl:Class ;
     rdfs:subClassOf :ProductionEntity ;
     rdfs:comment "Instruction to execute a specific operation on an object."@en .


###  http://example.org/def/production-trace-patterns/Machine
:Machine rdf:type owl:Class ;
         rdfs:subClassOf :Resource ;
         rdfs:comment "Resource that executes certain manufacturing operations."@en .


###  http://example.org/def/production-trace-patterns/Maintenance
:Maintenance rdf:type owl:Class ;
             rdfs:subClassOf :Event ;
             rdfs:comment "Describes the occasion when a Resource, in contrast to Repair this is often done before a Resource breaks."@en .


###  http://example.org/def/production-trace-patterns/MaterialLot
:MaterialLot rdf:type owl:Class ;
             rdfs:subClassOf :ProductionEntity ;
             rdfs:comment "Set of materials that are used in a process."@en .


###  http://example.org/def/production-trace-patterns/Merge
:Merge rdf:type owl:Class ;
       rdfs:subClassOf :Event ;
       rdfs:comment "Describes the occasion when the objects in one ProductionLot are transferred to another existing ProductionLot."@en .


###  http://example.org/def/production-trace-patterns/Observation
:Observation rdf:type owl:Class ;
             rdfs:subClassOf :Event ;
             rdfs:comment "Describes the occasion when for example a measurement is made by a Sensor."@en .


###  http://example.org/def/production-trace-patterns/Order
:Order rdf:type owl:Class ;
       rdfs:subClassOf :ProductionEntity ;
       rdfs:comment "Instruction to execute certain operations on certain objects."@en .


###  http://example.org/def/production-trace-patterns/Product
:Product rdf:type owl:Class ;
         rdfs:subClassOf :ProductionEntity ;
         rdfs:comment "Object that is a main result of a manufacturing process."@en .


###  http://example.org/def/production-trace-patterns/ProductionEntity
:ProductionEntity rdf:type owl:Class ;
                  rdfs:subClassOf :Entity ;
                  rdfs:comment "Entity that can be used to execute (parts of) a production process, for example a machine."@en .


###  http://example.org/def/production-trace-patterns/ProductionLot
:ProductionLot rdf:type owl:Class ;
               rdfs:subClassOf :ProductionEntity ;
               rdfs:comment "Set of objects that are handled together in a process."@en .


###  http://example.org/def/production-trace-patterns/Repair
:Repair rdf:type owl:Class ;
        rdfs:subClassOf :Event ;
        rdfs:comment "Describes the occasion that an Entity is repaired, for example the replacement of certain broken parts of a machine."@en .


###  http://example.org/def/production-trace-patterns/Resource
:Resource rdf:type owl:Class ;
          rdfs:subClassOf :Entity ;
          rdfs:comment "Entity that is the subject of a production process, for example a product."@en .


###  http://example.org/def/production-trace-patterns/Sensor
:Sensor rdf:type owl:Class ;
        rdfs:subClassOf :Entity ;
        rdfs:comment "Device that can be used to make observations."@en .


###  http://example.org/def/production-trace-patterns/SettingUp
:SettingUp rdf:type owl:Class ;
           rdfs:subClassOf :State .


###  http://example.org/def/production-trace-patterns/Split
:Split rdf:type owl:Class ;
       rdfs:subClassOf :Event ;
       rdfs:comment "Describes the occasion when a subset of the objects in one ProductionLot are transferred to another ProductionLot."@en .


###  http://example.org/def/production-trace-patterns/State
:State rdf:type owl:Class ;
       rdfs:comment "State in which a resource can be."@en .


###  http://example.org/def/production-trace-patterns/SwitchState
:SwitchState rdf:type owl:Class ;
             rdfs:subClassOf :Event ;
             rdfs:comment "Describes the occasion when a Resource changes to another state, for clarification also a set of typical machine states are included."@en .


###  http://example.org/def/production-trace-patterns/SwitchTool
:SwitchTool rdf:type owl:Class ;
            rdfs:subClassOf :Event ;
            rdfs:comment "Describes the occasion when a Resource changes to another Tool."@en .


###  http://example.org/def/production-trace-patterns/Tool
:Tool rdf:type owl:Class ;
      rdfs:subClassOf :Resource ;
      rdfs:comment "Resource that is used to execute specific manufacturing operations, for example a tool for grinding."@en .


###  http://example.org/def/production-trace-patterns/TrackIn
:TrackIn rdf:type owl:Class ;
         rdfs:subClassOf :Event ;
         rdfs:comment """Describes the occasion when a ProductionEntity is checked in at a Resource. For example, for a Machine we define this as the moment it starts processing the
ProductionEntity, and for a Buffer the arrival of a ProductionEntity."""@en .


###  http://example.org/def/production-trace-patterns/TrackOut
:TrackOut rdf:type owl:Class ;
          rdfs:subClassOf :Event ;
          rdfs:comment "Describes the occasion when a ProductionEntity is checked out at a Resource. For example, for a Machine we define this as the moment it finishes processing the ProductionEntity, and for a Buffer the departure of a ProductionEntity."@en .


###  http://example.org/def/production-trace-patterns/Working
:Working rdf:type owl:Class ;
         rdfs:subClassOf :State .


###  http://example.org/def/production-trace-patterns/Workstation
:Workstation rdf:type owl:Class ;
             rdfs:subClassOf :Resource ;
             rdfs:comment "Location at a shop floor where operations are executed, this can be done by different machines that are located in that workstation or by human workers."@en .


#################################################################
#    General axioms
#################################################################

[ rdf:type owl:AllDisjointClasses ;
  owl:members ( :AGV
                :Buffer
                :Machine
                :Tool
                :Workstation
              )
] .


[ rdf:type owl:AllDisjointClasses ;
  owl:members ( :Consume
                :Maintenance
                :Merge
                :Observation
                :Repair
                :Split
                :SwitchState
                :SwitchTool
                :TrackIn
                :TrackOut
              )
] .


[ rdf:type owl:AllDisjointClasses ;
  owl:members ( :Failed
                :Idle
                :SettingUp
                :Working
              )
] .


[ rdf:type owl:AllDisjointClasses ;
  owl:members ( :Job
                :MaterialLot
                :Order
                :Product
                :ProductionLot
              )
] .


[ rdf:type owl:AllDisjointClasses ;
  owl:members ( :ProductionEntity
                :Resource
                :Sensor
              )
] .


###  Generated by the OWL API (version 4.5.9.2019-02-01T07:24:44Z) https://github.com/owlcs/owlapi
